src/SDK/MessageHeader/Serialize.dfy
@@ -1,30 +1,29 @@
 include "Format.dfy"
+include "../Materials.dfy"
 include "../AlgorithmSuite.dfy"
 
 include "../../Util/Streams.dfy"
 include "../../StandardLibrary/StandardLibrary.dfy"
 
 module MessageHeader.Serialize {
-  import Msg = Definitions
-  import SerializeAAD
-  import SerializeEDK
-  import V = Validity
+  import Msg = Format
   import AlgorithmSuite
 
   import Streams
   import opened StandardLibrary
   import opened UInt = StandardLibrary.UInt
+  import Materials
 
   function {:opaque} Serialize(hb: Msg.HeaderBody): seq<uint8>
-    requires V.ValidHeaderBody(hb)
+    requires hb.Valid()
   {
-    reveal V.ValidHeaderBody();
+    //reveal Msg.HeaderBody.Valid();
     [hb.version as uint8] +
     [hb.typ as uint8] +
     UInt16ToSeq(hb.algorithmSuiteID as uint16) +
     hb.messageID +
-    SerializeAAD.SerializeAAD(hb.aad) +
-    SerializeEDK.SerializeEDKs(hb.encryptedDataKeys) +
+    SerializeAAD(hb.aad) +
+    SerializeEDKs(hb.encryptedDataKeys) +
     [Msg.ContentTypeToUInt8(hb.contentType)] +
     hb.reserved +
     [hb.ivLength] +
@@ -32,7 +31,7 @@ module MessageHeader.Serialize {
   }
 
   method SerializeHeaderBody(wr: Streams.StringWriter, hb: Msg.HeaderBody) returns (ret: Result<nat>)
-    requires wr.Valid() && V.ValidHeaderBody(hb)
+    requires wr.Valid() && hb.Valid()
     modifies wr`data
     ensures wr.Valid()
     ensures match ret
@@ -59,11 +58,11 @@ module MessageHeader.Serialize {
     len :- wr.WriteSimpleSeq(hb.messageID);
     totalWritten := totalWritten + len;
 
-    reveal V.ValidHeaderBody();
-    len :- SerializeAAD.SerializeAADImpl(wr, hb.aad);
+    //reveal Msg.HeaderBody.Valid();
+    len :- SerializeAADImpl(wr, hb.aad);
     totalWritten := totalWritten + len;
 
-    len :- SerializeEDK.SerializeEDKsImpl(wr, hb.encryptedDataKeys);
+    len :- SerializeEDKsImpl(wr, hb.encryptedDataKeys);
     totalWritten := totalWritten + len;
 
     var contentType := Msg.ContentTypeToUInt8(hb.contentType);
@@ -86,7 +85,7 @@ module MessageHeader.Serialize {
 
   method SerializeHeaderAuthentication(wr: Streams.StringWriter, ha: Msg.HeaderAuthentication, ghost algorithmSuiteID: AlgorithmSuite.ID) returns (ret: Result<nat>)
     requires wr.Valid()
-    requires V.ValidHeaderAuthentication(ha, algorithmSuiteID)
+    requires ha.Valid(algorithmSuiteID)
     modifies wr`data
     ensures wr.Valid()
     ensures match ret
@@ -102,24 +101,14 @@ module MessageHeader.Serialize {
     var n :- wr.WriteSimpleSeq(ha.authenticationTag);
     return Success(m + n);
   }
-}
 
-
-module MessageHeader.SerializeAAD {
-  import V = Validity
-  import Materials
-
-  import Streams
-  import opened StandardLibrary
-  import opened UInt = StandardLibrary.UInt
-
-  // ----- Specification -----
+  // ----- SerializeAAD Specification -----
 
   function SerializeAAD(kvPairs: Materials.EncryptionContext): seq<uint8>
-    requires V.ValidAAD(kvPairs)
+    requires Msg.ValidAAD(kvPairs)
   {
-    reveal V.ValidAAD();
-    UInt16ToSeq(V.AADLength(kvPairs) as uint16) +
+    reveal Msg.ValidAAD();
+    UInt16ToSeq(Msg.AADLength(kvPairs) as uint16) +
     var n := |kvPairs|;
     if n == 0 then [] else
       UInt16ToSeq(n as uint16) +
@@ -127,27 +116,27 @@ module MessageHeader.SerializeAAD {
   }
 
   function SerializeKVPairs(kvPairs: Materials.EncryptionContext, lo: nat, hi: nat): seq<uint8>
-    requires forall i :: 0 <= i < |kvPairs| ==> V.ValidKVPair(kvPairs[i])
+    requires forall i :: 0 <= i < |kvPairs| ==> Msg.ValidKVPair(kvPairs[i])
     requires lo <= hi <= |kvPairs|
   {
     if lo == hi then [] else SerializeKVPairs(kvPairs, lo, hi - 1) + SerializeKVPair(kvPairs[hi - 1])
   }
 
   function SerializeKVPair(kvPair: (seq<uint8>, seq<uint8>)): seq<uint8>
-    requires V.ValidKVPair(kvPair)
+    requires Msg.ValidKVPair(kvPair)
   {
     UInt16ToSeq(|kvPair.0| as uint16) + kvPair.0 +
     UInt16ToSeq(|kvPair.1| as uint16) + kvPair.1
   }
 
-  // Function V.AADLength is defined without referring to SerializeAAD (because then
-  // these two would be mutually recursive with V.ValidAAD). The following lemma proves
+  // Function Msg.AADLength is defined without referring to SerializeAAD (because then
+  // these two would be mutually recursive with Msg.ValidAAD). The following lemma proves
   // that the two definitions correspond.
   lemma ADDLengthCorrect(kvPairs: Materials.EncryptionContext)
-    requires V.ValidAAD(kvPairs)
-    ensures |SerializeAAD(kvPairs)| == 2 + V.AADLength(kvPairs)
+    requires Msg.ValidAAD(kvPairs)
+    ensures |SerializeAAD(kvPairs)| == 2 + Msg.AADLength(kvPairs)
   {
-    reveal V.ValidAAD();
+    reveal Msg.ValidAAD();
     KVPairsLengthCorrect(kvPairs, 0, |kvPairs|);
     /**** Here's a more detailed proof:
     var n := |kvPairs|;
@@ -156,20 +145,20 @@ module MessageHeader.SerializeAAD {
       calc {
         |SerializeAAD(kvPairs)|;
       ==  // def. SerializeAAD
-        |UInt16ToSeq(V.AADLength(kvPairs) as uint16) + UInt16ToSeq(n as uint16) + s|;
+        |UInt16ToSeq(Msg.AADLength(kvPairs) as uint16) + UInt16ToSeq(n as uint16) + s|;
       ==  // UInt16ToSeq yields length-2 sequence
         2 + 2 + |s|;
       ==  { KVPairsLengthCorrect(kvPairs, 0, n); }
-        2 + 2 + V.KVPairsLength(kvPairs, 0, n);
+        2 + 2 + Msg.KVPairsLength(kvPairs, 0, n);
       }
     }
     ****/
   }
 
   lemma KVPairsLengthCorrect(kvPairs: Materials.EncryptionContext, lo: nat, hi: nat)
-    requires forall i :: 0 <= i < |kvPairs| ==> V.ValidKVPair(kvPairs[i])
+    requires forall i :: 0 <= i < |kvPairs| ==> Msg.ValidKVPair(kvPairs[i])
     requires lo <= hi <= |kvPairs|
-    ensures |SerializeKVPairs(kvPairs, lo, hi)| == V.KVPairsLength(kvPairs, lo, hi)
+    ensures |SerializeKVPairs(kvPairs, lo, hi)| == Msg.KVPairsLength(kvPairs, lo, hi)
   {
     /**** Here's a more detailed proof:
     if lo < hi {
@@ -181,25 +170,25 @@ module MessageHeader.SerializeAAD {
       ==
         |SerializeKVPairs(kvPairs, lo, hi - 1)| + |SerializeKVPair(kvPair)|;
       ==  { KVPairsLengthCorrect(kvPairs, lo, hi - 1); }
-        V.KVPairsLength(kvPairs, lo, hi - 1) + |SerializeKVPair(kvPair)|;
+        Msg.KVPairsLength(kvPairs, lo, hi - 1) + |SerializeKVPair(kvPair)|;
       ==  // def. SerializeKVPair
-        V.KVPairsLength(kvPairs, lo, hi - 1) +
+        Msg.KVPairsLength(kvPairs, lo, hi - 1) +
         |UInt16ToSeq(|kvPair.0| as uint16) + kvPair.0 + UInt16ToSeq(|kvPair.1| as uint16) + kvPair.1|;
       ==
-        V.KVPairsLength(kvPairs, lo, hi - 1) + 2 + |kvPair.0| + 2 + |kvPair.1|;
-      ==  // def. V.KVPairsLength
-        V.KVPairsLength(kvPairs, lo, hi);
+        Msg.KVPairsLength(kvPairs, lo, hi - 1) + 2 + |kvPair.0| + 2 + |kvPair.1|;
+      ==  // def. Msg.KVPairsLength
+        Msg.KVPairsLength(kvPairs, lo, hi);
       }
     }
     ****/
   }
 
-  // ----- Implementation -----
+  // ----- SerializeAAD Implementation -----
 
   method SerializeAADImpl(wr: Streams.StringWriter, kvPairs: Materials.EncryptionContext) returns (ret: Result<nat>)
-    requires wr.Valid() && V.ValidAAD(kvPairs)
+    requires wr.Valid() && Msg.ValidAAD(kvPairs)
     modifies wr`data
-    ensures wr.Valid() && V.ValidAAD(kvPairs)
+    ensures wr.Valid() && Msg.ValidAAD(kvPairs)
     ensures match ret
       case Success(totalWritten) =>
         var serAAD := SerializeAAD(kvPairs);
@@ -209,7 +198,7 @@ module MessageHeader.SerializeAAD {
         && wr.data == old(wr.data) + serAAD
       case Failure(e) => true
   {
-    reveal V.ValidAAD();
+    reveal Msg.ValidAAD();
     var totalWritten := 0;
 
     // Key Value Pairs Length (number of bytes of total AAD)
@@ -260,10 +249,10 @@ module MessageHeader.SerializeAAD {
 
   method ComputeAADLength(kvPairs: Materials.EncryptionContext) returns (res: Result<uint16>)
     requires |kvPairs| < UINT16_LIMIT
-    requires forall i :: 0 <= i < |kvPairs| ==> V.ValidKVPair(kvPairs[i])
+    requires forall i :: 0 <= i < |kvPairs| ==> Msg.ValidKVPair(kvPairs[i])
     ensures match res
-      case Success(len) => len as int == V.AADLength(kvPairs)
-      case Failure(_) => UINT16_LIMIT <= V.AADLength(kvPairs)
+      case Success(len) => len as int == Msg.AADLength(kvPairs)
+      case Failure(_) => UINT16_LIMIT <= Msg.AADLength(kvPairs)
   {
     var n: int32 := |kvPairs| as int32;
     if n == 0 {
@@ -273,11 +262,11 @@ module MessageHeader.SerializeAAD {
       var i: int32 := 0;
       while i < n
         invariant i <= n
-        invariant 2 + V.KVPairsLength(kvPairs, 0, i as int) == len as int < UINT16_LIMIT
+        invariant 2 + Msg.KVPairsLength(kvPairs, 0, i as int) == len as int < UINT16_LIMIT
       {
         var kvPair := kvPairs[i];
         len := len + 4 + |kvPair.0| as int32 + |kvPair.1| as int32;
-        V.KVPairsLengthSplit(kvPairs, 0, i as int + 1, n as int);
+        Msg.KVPairsLengthSplit(kvPairs, 0, i as int + 1, n as int);
         if limit <= len {
           return Failure("The number of bytes in encryption context exceeds the allowed maximum");
         }
@@ -286,24 +275,13 @@ module MessageHeader.SerializeAAD {
       return Success(len as uint16);
     }
   }
-}
 
-
-module MessageHeader.SerializeEDK {
-  import Msg = Definitions
-  import V = Validity
-  import Materials
-
-  import Streams
-  import opened StandardLibrary
-  import opened UInt = StandardLibrary.UInt
-
-  // ----- Specification -----
+  // ----- SerializeEDKs Specification -----
 
   function SerializeEDKs(encryptedDataKeys: Msg.EncryptedDataKeys): seq<uint8>
-    requires V.ValidEncryptedDataKeys(encryptedDataKeys)
+    requires encryptedDataKeys.Valid()
   {
-    reveal V.ValidEncryptedDataKeys();
+    //reveal Msg.EncryptedDataKeys.Valid();
     var n := |encryptedDataKeys.entries|;
     UInt16ToSeq(n as uint16) +
     SerializeEDKEntries(encryptedDataKeys.entries, 0, n)
@@ -324,12 +302,12 @@ module MessageHeader.SerializeEDK {
     UInt16ToSeq(|edk.ciphertext| as uint16)   + edk.ciphertext
   }
 
-  // ----- Implementation -----
+  // ----- SerializeEDKs Implementation -----
 
   method SerializeEDKsImpl(wr: Streams.StringWriter, encryptedDataKeys: Msg.EncryptedDataKeys) returns (ret: Result<nat>)
-    requires wr.Valid() && V.ValidEncryptedDataKeys(encryptedDataKeys)
+    requires wr.Valid() && encryptedDataKeys.Valid()
     modifies wr`data
-    ensures wr.Valid() && V.ValidEncryptedDataKeys(encryptedDataKeys)
+    ensures wr.Valid() && encryptedDataKeys.Valid()
     ensures match ret
       case Success(totalWritten) =>
         var serEDK := SerializeEDKs(encryptedDataKeys);
@@ -339,7 +317,7 @@ module MessageHeader.SerializeEDK {
         && wr.data == old(wr.data) + serEDK
       case Failure(e) => true
   {
-    reveal V.ValidEncryptedDataKeys();
+    //reveal Msg.EncryptedDataKeys.Valid();
 
     var totalWritten := 0;
 
